added support for container of

examples/container_of.c
@@ -1,0 +1,17 @@
+
+#define container_of(ptr, type, member) (type *)( (char *)(ptr) - offsetof(type,member) )
+
+struct test {
+  int a;
+  int b;
+};
+
+[[rc::returns("{4} @ int<i32>")]]
+int container_of_test() {
+  struct test t = {.a = 1, .b = 2};
+  int *b = &t.b;
+  *b = 3;
+  struct test *pt = container_of(b, struct test, b);
+  pt->a = 4;
+  return pt->a;
+}
