examples/proofs/container_of/generated_code.v
@@ -1,0 +1,80 @@
+From refinedc.lang Require Export notation.
+From refinedc.lang Require Import tactics.
+From refinedc.typing Require Import annotations.
+Set Default Proof Using "Type".
+
+(* Generated from [examples/container_of.c]. *)
+Section code.
+  Definition file_0 : string := "examples/container_of.c".
+  Definition loc_2 : location_info := LocationInfo file_0 11 2 11 35.
+  Definition loc_3 : location_info := LocationInfo file_0 12 2 12 16.
+  Definition loc_4 : location_info := LocationInfo file_0 13 2 13 9.
+  Definition loc_5 : location_info := LocationInfo file_0 14 2 14 77.
+  Definition loc_6 : location_info := LocationInfo file_0 15 2 15 12.
+  Definition loc_7 : location_info := LocationInfo file_0 16 2 16 15.
+  Definition loc_8 : location_info := LocationInfo file_0 16 9 16 14.
+  Definition loc_9 : location_info := LocationInfo file_0 16 9 16 14.
+  Definition loc_10 : location_info := LocationInfo file_0 16 9 16 11.
+  Definition loc_11 : location_info := LocationInfo file_0 16 9 16 11.
+  Definition loc_12 : location_info := LocationInfo file_0 15 2 15 7.
+  Definition loc_13 : location_info := LocationInfo file_0 15 2 15 4.
+  Definition loc_14 : location_info := LocationInfo file_0 15 2 15 4.
+  Definition loc_15 : location_info := LocationInfo file_0 15 10 15 11.
+  Definition loc_16 : location_info := LocationInfo file_0 14 20 14 76.
+  Definition loc_17 : location_info := LocationInfo file_0 14 35 14 76.
+  Definition loc_18 : location_info := LocationInfo file_0 14 37 14 48.
+  Definition loc_19 : location_info := LocationInfo file_0 14 45 14 48.
+  Definition loc_20 : location_info := LocationInfo file_0 14 45 14 48.
+  Definition loc_21 : location_info := LocationInfo file_0 14 51 14 74.
+  Definition loc_24 : location_info := LocationInfo file_0 13 2 13 4.
+  Definition loc_25 : location_info := LocationInfo file_0 13 3 13 4.
+  Definition loc_26 : location_info := LocationInfo file_0 13 3 13 4.
+  Definition loc_27 : location_info := LocationInfo file_0 13 7 13 8.
+  Definition loc_28 : location_info := LocationInfo file_0 12 11 12 15.
+  Definition loc_29 : location_info := LocationInfo file_0 12 12 12 15.
+  Definition loc_30 : location_info := LocationInfo file_0 12 12 12 13.
+  Definition loc_34 : location_info := LocationInfo file_0 11 32 11 33.
+  Definition loc_35 : location_info := LocationInfo file_0 11 24 11 25.
+
+  (* Definition of struct [test]. *)
+  Program Definition struct_test := {|
+    sl_members := [
+      (Some "a", it_layout i32);
+      (Some "b", it_layout i32)
+    ];
+  |}.
+  Solve Obligations with solve_struct_obligations.
+
+  (* Definition of function [container_of_test]. *)
+  Definition impl_container_of_test : function := {|
+    f_args := [
+    ];
+    f_local_vars := [
+      ("b", LPtr);
+      ("t", layout_of struct_test);
+      ("pt", LPtr)
+    ];
+    f_init := "#0";
+    f_code := (
+      <[ "#0" :=
+        "t" <-{ layout_of struct_test }
+          StructInit struct_test [
+            ("a", LocInfoE loc_35 (i2v 1 i32) : expr) ;
+            ("b", LocInfoE loc_34 (i2v 2 i32) : expr)
+          ] ;
+        "b" <-{ LPtr }
+          LocInfoE loc_28 (&(LocInfoE loc_29 ((LocInfoE loc_30 ("t")) at{struct_test} "b"))) ;
+        locinfo: loc_4 ;
+        LocInfoE loc_25 (!{LPtr} (LocInfoE loc_26 ("b"))) <-{ it_layout i32 }
+          LocInfoE loc_27 (i2v 3 i32) ;
+        "pt" <-{ LPtr }
+          LocInfoE loc_16 (UnOp (CastOp $ PtrOp) (PtrOp) (LocInfoE loc_17 ((LocInfoE loc_18 (UnOp (CastOp $ PtrOp) (PtrOp) (LocInfoE loc_19 (use{LPtr} (LocInfoE loc_20 ("b")))))) at_neg_offset{it_layout u8, PtrOp, IntOp size_t} (LocInfoE loc_21 ((OffsetOf (struct_test) ("b"))))))) ;
+        locinfo: loc_6 ;
+        LocInfoE loc_12 ((LocInfoE loc_13 (!{LPtr} (LocInfoE loc_14 ("pt")))) at{struct_test} "a") <-{ it_layout i32 }
+          LocInfoE loc_15 (i2v 4 i32) ;
+        locinfo: loc_7 ;
+        Return (LocInfoE loc_8 (use{it_layout i32} (LocInfoE loc_9 ((LocInfoE loc_10 (!{LPtr} (LocInfoE loc_11 ("pt")))) at{struct_test} "a"))))
+      ]> $∅
+    )%E
+  |}.
+End code.
