examples/proofs/container_of/generated_proof_container_of_test.v
@@ -1,0 +1,25 @@
+From refinedc.typing Require Import typing.
+From refinedc.examples.container_of Require Import generated_code.
+From refinedc.examples.container_of Require Import generated_spec.
+Set Default Proof Using "Type".
+
+(* Generated from [examples/container_of.c]. *)
+Section proof_container_of_test.
+  Context `{!typeG Σ} `{!globalG Σ}.
+
+  (* Typing proof for [container_of_test]. *)
+  Lemma type_container_of_test :
+    ⊢ typed_function impl_container_of_test type_of_container_of_test.
+  Proof.
+    start_function "container_of_test" ([]) => local_b local_t local_pt.
+    split_blocks ((
+      ∅
+    )%I : gmap label (iProp Σ)) ((
+      ∅
+    )%I : gmap label (iProp Σ)).
+    - repeat liRStep; liShow.
+      all: print_typesystem_goal "container_of_test" "#0".
+    Unshelve. all: sidecond_hook; prepare_sideconditions; normalize_and_simpl_goal; try solve_goal; unsolved_sidecond_hook.
+    all: print_sidecondition_goal "container_of_test".
+  Qed.
+End proof_container_of_test.
