examples/proofs/container_of/generated_spec.v
@@ -1,0 +1,14 @@
+From refinedc.typing Require Import typing.
+From refinedc.examples.container_of Require Import generated_code.
+Set Default Proof Using "Type".
+
+(* Generated from [examples/container_of.c]. *)
+Section spec.
+  Context `{!typeG Σ} `{!globalG Σ}.
+
+  (* Type definitions. *)
+
+  (* Specifications for function [container_of_test]. *)
+  Definition type_of_container_of_test :=
+    fn(∀ () : (); True) → ∃ () : (), ((4) @ (int (i32))); True.
+End spec.
