theories/lang/lang.v
@@ -288,7 +288,7 @@ Inductive bin_op : Set :=
 | AddOp | SubOp | MulOp | DivOp | ModOp | AndOp | OrOp | XorOp | ShlOp
 | ShrOp | EqOp | NeOp | LtOp | GtOp | LeOp | GeOp
 (* Ptr is the second argument and pffset the first *)
-| PtrOffsetOp (ly : layout).
+| PtrOffsetOp (ly : layout) | PtrNegOffsetOp (ly : layout).
 
 Inductive un_op : Set :=
 | NotBoolOp | NotIntOp | NegOp | CastOp (ot : op_type).
@@ -756,6 +756,11 @@ Inductive eval_bin_op : bin_op → op_type → op_type → state → val → val
     (* TODO: should we have an alignment check here? *)
     0 ≤ o →
     eval_bin_op (PtrOffsetOp ly) (IntOp it) PtrOp σ v1 v2 (val_of_loc (l offset{ly}ₗ o))
+| PtrNegOffsetOpIP v1 v2 σ o l ly it:
+    val_to_int v1 it = Some o →
+    val_to_loc v2 = Some l →
+    (* TODO: should we have an alignment check here? *)
+    eval_bin_op (PtrNegOffsetOp ly) (IntOp it) PtrOp σ v1 v2 (val_of_loc (l offset{ly}ₗ -o))
 | EqOpPNull v1 v2 σ l v:
     heap_loc_in_bounds l 0%nat σ →
     val_to_loc v1 = Some l →
